%-*-latex-*-
 
\qed
We will attempt to prove the following via weak mathematical induction:

\[ 4(1^3 + 2^3 + \dots + n^3) = n^2(n + 1)^2, \forall n \geq 1 \]

\textsc{Base Case}:

With $n = 1$ in $P(n)$ we have

\[ P(1) = 4(1^3 + 2^3 + \dots + n^3) = 4(1^3), n^2(n + 1)^2 = 1^3(1 + 1)^2 \]
\[ 4(1^3) = 4, 1^3(1 + 1)^2 = 1(2)^2 = 1(4) = 4 \]

We have shown $P(1)$ holds.

\textsc{Inductive Case}:
Now we will attempt to prove $P(n)$ for all $n \geq 1$.

  \[ P(n + 1) = 4(1^3 + 2^3 + \dots + n^3 + (n + 1)^3) = (\textbf{n + 1})^2( (\textbf{n + 1}) + 1)^2 \]

We begin by factoring out squares from the sum on the left hand side, making it appear like

\[ 4(1 + 2 + \dots + n + (n + 1) )^2 \]

which takes the same form as an arithmetic sum. Rewriting the LHS we get


\[ 4(\frac{(n + 1)( (n + 1) + 1)^2}{2})^2 \]

\[ 4(\frac{(n + 1)( (n + 1) + 1) \cdot (n + 1)( (n + 1) + 1)}{2 \cdot 2}) \]

\[ (n + 1)( (n + 1) + 1) \cdot (n + 1)( (n + 1) + 1) \]

\[ (n + 1)^2( (n + 1) + 1)^2 \]

\qedsymbol{}
